The point (1, -2) is on the graph of \( f \). Describe the following transformations on \( f \), and determine the resulting point.

We use
\[
g(x) = a f(k(x - d)) + c,
\quad
x' = \frac{x}{k} + d,
\quad
y' = a y + c.
\]

a) \( g(x) = 2f(x) + 3 \)

The \( a = 2 \) indicates a vertical stretch by a factor of 2 and the \( c = 3 \) indicates a vertical translation of 3 units up.
\[
\begin{align*}
x' &= \frac{x}{k} + d \\
&= \frac{1}{1} + 0 \\
&= 1 \\
y' &= a y + c \\
&= 2(-2) + 3 \\
&= -1
\end{align*}
\]

Therefore, the resulting point is \( \boxed{(1, -1)} \).