a) p(r) = 2r2 + 2r −1
x = 2y2 + 2y −1
x + 1 = 2
(
y2 + y
)
x + 1 = 2
[(
y + 1
2
)2
−1
4
]
x + 1 = 2
(
y + 1
2
)2
−1
2
x + 3
2 = 2
(
y + 1
2
)2
x
2 + 3
4 =
(
y + 1
2
)2
y + 1
2 = ±
√
x
2 + 3
4
y = −1
2 ±
√
x
2 + 3
4
p−1(x) =−1
2 ±
√
x
2 + 3
4
b) 3y + 5x = 18
3y + 5x = 18
3y = −5x + 18
y = −5
3 x + 6
x = −5
3 y + 6
x −6 =−5
3 y
y = −3
5 (x −6)
y = −3
5 x + 18
5
f−1(x) =−3
5 x + 18
5
c) h(t) =−4.9(t + 3)2 + 45.8
x = −4.9(y + 3)2 + 45.8
x −45.8 =−4.9(y + 3)2
45.8 −x = 4.9(y + 3)2
45.8 −x
4.9 = (y + 3)2
y + 3 =±
√
45.8 −x
4.9
y = −3 ±
√
45.8 −x
4.9
h−1(x) =−3 ±
√
45.8 −x
4.9
2