b) g(x) =f(x + 1)−3
The d = −1 (since x −d = x −(−1) =x + 1) indicates a horizontal translation of1 unit to the left
and thec = −3 indicates a vertical translation of3 units down.
x′= x
k + d
= 1
1 + (−1)
= 0
y′= a y+ c
= 1(−2) + (−3)
= −5
Therefore, the resulting point is(0, −5) .
c) g(x) =−f(2x)
The a = −1 indicates a reflection in thex-axis and thek = 2indicates a horizontal compression by
a factor of1/2.
x′= x
k + d
= 1
2 + 0
= 1
2
y′= a y+ c
= (−1)(−2) + 0
= 2
Therefore, the resulting point is
(1
2 , 2
)
.
7